cannot get the internal mem_mgr to entail the general mem_mgr

kalloc/kalloc.h
@@ -1,0 +1,2 @@
+void*           kalloc(void);
+void            kfree(void *);
