kalloc/ASI_kalloc.v
@@ -16,7 +16,15 @@ Record KallocTokenAPD := {
 
 Record KallocFreeAPD := {
   KF_Tok :> KallocTokenAPD;   (* whenever KallocFreeAPD is used, but a KallocTokenAPD is expected, it is automatically converted *)
-  mem_mgr: globals -> share -> list val -> Z -> val -> mpred;
+  mem_mgr: globals -> mpred;
+  mem_mgr_local_facts: forall gv,
+    (mem_mgr gv) |-- (EX (sh : share), EX (ls: list val), EX (original_freelist_pointer:val), (* I am unsure how to access all these elements.. *)
+      !! (writable_share sh /\
+        is_pointer_or_null original_freelist_pointer /\
+              (((ls = nil) /\ original_freelist_pointer = nullval) \/ 
+              ((ls <> nil) /\ isptr original_freelist_pointer))
+        ))
+
 }.
 
 #[export] Hint Resolve kalloc_token'_valid_pointer : valid_pointer. 
@@ -32,14 +40,14 @@ Variable kfreeID: ident.
 
 Definition kfree_spec' := 
   DECLARE kfreeID
-      WITH n:Z, new_head:val, gv:globals, sh:share, ls: list val, xx:Z, original_freelist_pointer:val
+      WITH n:Z, new_head:val, gv:globals, sh:share
       PRE [ tptr tvoid]
         PROP(
               is_pointer_or_null new_head
               ) 
         PARAMS (new_head) GLOBALS(gv)
         SEP (
-          mem_mgr K gv sh ls xx original_freelist_pointer;
+          mem_mgr K gv;
           if eq_dec new_head nullval then emp
           else (kalloc_token' K sh (n) new_head (* memory_block Ews n new_head*))
         )
@@ -48,33 +56,28 @@ Definition kfree_spec' :=
         RETURN () 
         SEP (
           if eq_dec new_head nullval then 
-          mem_mgr K gv sh ls xx original_freelist_pointer
+          mem_mgr K gv
           else 
-            mem_mgr K gv sh (original_freelist_pointer::ls) xx new_head
+            mem_mgr K gv
             ).
 
 
 Definition kalloc_spec' :=
 DECLARE kallocID
-WITH n:Z, gv:globals, sh:share, ls: list val, xx:Z, original_freelist_pointer:val
+WITH n:Z, gv:globals, sh:share
 PRE [ ]
     PROP(0 <= n <= PGSIZE) 
     PARAMS () GLOBALS(gv)
-    SEP ( mem_mgr K gv sh ls xx original_freelist_pointer )  
-POST [ tptr tvoid ]
+    SEP ( mem_mgr K gv )  
+POST [ tptr tvoid ] EX p:_,
     PROP()
-    RETURN (original_freelist_pointer) 
+    RETURN (p) 
     SEP (
-      if (eq_dec original_freelist_pointer nullval) then
-        (mem_mgr K gv sh ls xx original_freelist_pointer * emp)
+      if (eq_dec p nullval) then
+        (mem_mgr K gv * emp)
       else 
-        (
-          EX next ls',
-          (!! (next :: ls' = ls) &&
-              kalloc_token' K sh n original_freelist_pointer *
-              mem_mgr K gv sh ls' xx next
-          )
-        )
+        kalloc_token' K sh n p *
+        mem_mgr K gv
     ).
 
 Definition Kalloc_ASI:funspecs := [kalloc_spec'; kfree_spec'].
