kalloc/Spec_kalloc.v
@@ -96,7 +96,7 @@ Definition kfree_spec (K:KallocFreeAPD) {cs: compspecs} (t: type) :=
               ) 
         PARAMS (new_head) GLOBALS(gv)
         SEP (
-          ASI_kalloc.mem_mgr K gv sh ls xx original_freelist_pointer *
+          mem_mgr_internal gv sh ls xx original_freelist_pointer *
           (if eq_dec new_head nullval then emp
           else (type_kalloc_token K sh (t) new_head))
         )
@@ -105,32 +105,32 @@ Definition kfree_spec (K:KallocFreeAPD) {cs: compspecs} (t: type) :=
         RETURN () 
         SEP (
           if eq_dec new_head nullval then 
-          ASI_kalloc.mem_mgr K gv sh ls xx original_freelist_pointer
+          mem_mgr_internal gv sh ls xx original_freelist_pointer
           else 
-          ASI_kalloc.mem_mgr K gv sh (original_freelist_pointer::ls) xx new_head
+          mem_mgr_internal gv sh (original_freelist_pointer::ls) xx new_head
             ).
 
-Definition kalloc_spec (K:KallocFreeAPD) {cs: compspecs} (t: type) :=
+Definition kalloc_spec (K:KallocFreeAPD) {cs: compspecs} (t: type) (ls:list val) (xx:Z) (original_freelist_pointer:val) :=
 DECLARE _kalloc
-WITH gv:globals, sh:share, ls: list val, xx:Z, original_freelist_pointer:val
+WITH gv:globals, sh:share(*, ls: list val, xx:Z, original_freelist_pointer:val*)
 PRE [ ]
     PROP(0 <= (sizeof t) <= PGSIZE;
             complete_legal_cosu_type t = true;
             natural_aligned natural_alignment t = true) 
     PARAMS () GLOBALS(gv)
-    SEP ( ASI_kalloc.mem_mgr K gv sh ls xx original_freelist_pointer )  
+    SEP ( mem_mgr_internal gv sh ls xx original_freelist_pointer )  
 POST [ tptr tvoid ]
     PROP()
     RETURN (original_freelist_pointer) 
     SEP (
       if (eq_dec original_freelist_pointer nullval) then
-        (ASI_kalloc.mem_mgr K gv sh ls xx original_freelist_pointer * emp)
+        (mem_mgr_internal gv sh ls xx original_freelist_pointer * emp)
       else 
         (
           EX next ls',
           (!! (next :: ls' = ls) &&
               type_kalloc_token K sh t original_freelist_pointer *
-              ASI_kalloc.mem_mgr K gv sh ls' xx next
+              mem_mgr_internal gv sh ls' xx next
         )
         )
     ).
@@ -140,16 +140,49 @@ POST [ tptr tvoid ]
 (** ** How to use the type-based specification of kalloc and kfree *)
 
 Lemma kalloc_spec_sub:
+ forall (K:KallocFreeAPD) {cs: compspecs} (t: type)(ls:list val) (xx:Z) (original_freelist_pointer:val),
+   funspec_sub (snd (kalloc_spec' K _kalloc)) (snd (kalloc_spec K t ls xx original_freelist_pointer)).
+Proof.
+  do_funspec_sub.
+  destruct w as [gv sh].
+  Exists (sizeof t, gv, sh) emp.
+  Intros.
+  entailer!.
+  2: {
+    unfold mem_mgr_internal. entailer!.
+  }
+  unfold mem_mgr_internal.
+  destruct w as [[[[gv sh] ls] xx] original_freelist_pointer].
+  Exists (sizeof t, gv, sh) emp. entailer!.
+  intros tau ? ?. 
+  if_tac; auto.
+  
+  Exists (eval_id ret_temp tau).
+  entailer!.
+  if_tac; auto.
+  unfold malloc_token.
+  assert_PROP (field_compatible t [] (eval_id ret_temp tau)).
+  { entailer!.
+    apply malloc_compatible_field_compatible; auto. }
+  entailer!.
+  rewrite memory_block_data_at_; auto.
+Qed.
+
+Lemma kalloc_spec_sub:
   forall  (K:KallocFreeAPD) {cs: compspecs} (t: type), 
     funspec_sub (snd (kalloc_spec' K _kalloc)) (snd (kalloc_spec K t)).
   Proof.
     do_funspec_sub. 
     entailer.
-    destruct w.
-    repeat (destruct p).
-    Exists (sizeof t, g0, s, l, z, v) emp. entailer.
+    destruct w as [[[[gv sh] ls] xx] original_freelist_pointer].
+    Exists (sizeof t, gv, sh) emp. entailer!.
+    intros tau.
     if_tac.
-    - entailer!. entailer!.
+    - rewrite mem_mgr_internal_split. entailer!.
+    intros tau.
+    Exists (eval_id ret_temp rho').
+      destruct (EqDec_val x nullval)
+    rewrite (mem_mgr_external_split). entailer!.
     - entailer!.
       + entailer!. Exists next ls'. entailer!. unfold type_kalloc_token. 
       assert_PROP (field_compatible t [] (eval_id ret_temp x)).
